Add complicated example proof for composition and demotion
Also fix a ton of issues in the original axiomatization in the process

operations/BMV_Composition.thy
@@ -1,15 +1,465 @@
 theory BMV_Composition
   imports "Binders.MRBNF_Recursor"
+  keywords "print_pbmv_monads" :: diag and
+   "pbmv_monad" :: thy_goal
 begin
 
-binder_datatype 'a type = Var 'a | App "'a type" "'a type list" | Forall x::'a t::"'a type" binds x in t
+lemma image_const_empty: "x \<noteq> y \<Longrightarrow> (\<lambda>_. x) ` A = (\<lambda>_. y) ` B \<Longrightarrow> A = {} \<and> B = {}"
+  by fast
 
-abbreviation "bd_type \<equiv> natLeq"
+ML_file \<open>../Tools/bmv_monad_def.ML\<close>
 
-abbreviation "sb_type \<equiv> tvsubst_type"
+(* live, free, free, live, live, dead, free *)
+typedecl ('a, 'b, 'c, 'd, 'e, 'f, 'g) T1
+(* dead, free, dead, free *)
+typedecl ('a, 'b, 'c, 'd) T2
+(* free, free, free, live, dead, live *)
+typedecl ('a, 'b, 'c, 'd, 'e, 'f) T3
+(* free, live *)
+typedecl ('a, 'b) T4
 
+consts Sb_T1 :: "('b::var \<Rightarrow> 'b) \<Rightarrow> ('c::var \<Rightarrow> ('a, 'b, 'c, 'd, 'e, 'f, 'g) T1) \<Rightarrow> ('g::var \<Rightarrow> ('a, 'b, 'c, 'd, 'e, 'f, 'g) T1) \<Rightarrow> ('a, 'b, 'c, 'd, 'e, 'f, 'g) T1 \<Rightarrow> ('a, 'b, 'c, 'd, 'e, 'f, 'g) T1"
+consts Map_T1 :: "('a \<Rightarrow> 'a') \<Rightarrow> ('d \<Rightarrow> 'd') \<Rightarrow> ('e \<Rightarrow> 'e') \<Rightarrow> ('a, 'b::var, 'c::var, 'd, 'e, 'f, 'g::var) T1 \<Rightarrow> ('a', 'b, 'c, 'd', 'e', 'f, 'g) T1"
+consts set_1_T1 :: "('a, 'b::var, 'c::var, 'd, 'e, 'f, 'g::var) T1 \<Rightarrow> 'a set"
+consts set_2_T1 :: "('a, 'b::var, 'c::var, 'd, 'e, 'f, 'g::var) T1 \<Rightarrow> 'd set"
+consts set_3_T1 :: "('a, 'b::var, 'c::var, 'd, 'e, 'f, 'g::var) T1 \<Rightarrow> 'e set"
+consts Vrs_1_T1 :: "('a, 'b::var, 'c::var, 'd, 'e, 'f, 'g::var) T1 \<Rightarrow> 'b set"
+consts Vrs_2_T1 :: "('a, 'b::var, 'c::var, 'd, 'e, 'f, 'g::var) T1 \<Rightarrow> 'c set"
+consts Vrs_3_T1 :: "('a, 'b::var, 'c::var, 'd, 'e, 'f, 'g::var) T1 \<Rightarrow> 'g set"
+consts Inj_1_T1 :: "'c \<Rightarrow> ('a, 'b::var, 'c::var, 'd, 'e, 'f, 'g::var) T1"
+consts Inj_2_T1 :: "'g \<Rightarrow> ('a, 'b::var, 'c::var, 'd, 'e, 'f, 'g::var) T1"
 
-(* Comp *)
-type_synonym 'a T = "'a + 'a type"
+consts Sb_T2 :: "('d::var \<Rightarrow> 'd) \<Rightarrow> ('b::var \<Rightarrow> ('a, 'b, 'c, 'd) T2) \<Rightarrow> ('a, 'b, 'c, 'd) T2 \<Rightarrow> ('a, 'b, 'c, 'd) T2"
+consts Vrs_1_T2 :: "('a, 'b::var, 'c, 'd::var) T2 \<Rightarrow> 'd set"
+consts Vrs_2_T2 :: "('a, 'b::var, 'c, 'd::var) T2 \<Rightarrow> 'b set"
+consts Inj_T2 :: "'b \<Rightarrow> ('a, 'b::var, 'c, 'd::var) T2"
+
+consts Sb_T3 :: "('a::var \<Rightarrow> ('a::var, 'b, 'c::var, 'd, 'e, 'f) T3) \<Rightarrow> ('a::var \<Rightarrow> ('a::var, 'c::var) T4) \<Rightarrow> ('b::var \<Rightarrow> ('a::var, 'b, 'c::var, 'd, 'e, 'f) T3) \<Rightarrow> ('c::var \<Rightarrow> ('a, 'c) T4) \<Rightarrow> ('a::var, 'b, 'c::var, 'd, 'e, 'f) T3 \<Rightarrow> ('a::var, 'b, 'c::var, 'd, 'e, 'f) T3"
+consts Map_T3 :: "('d \<Rightarrow> 'd') \<Rightarrow> ('f \<Rightarrow> 'f') \<Rightarrow> ('a::var, 'b, 'c::var, 'd, 'e, 'f) T3 \<Rightarrow> ('a, 'b, 'c, 'd', 'e, 'f') T3"
+consts set_1_T3 :: "('a::var, 'b, 'c::var, 'd, 'e, 'f) T3 \<Rightarrow> 'd set"
+consts set_2_T3 :: "('a::var, 'b, 'c::var, 'd, 'e, 'f) T3 \<Rightarrow> 'f set"
+consts Vrs_1_T3 :: "('a::var, 'b, 'c::var, 'd, 'e, 'f) T3 \<Rightarrow> 'a set"
+consts Vrs_2_T3 :: "('a::var, 'b, 'c::var, 'd, 'e, 'f) T3 \<Rightarrow> 'a set"
+consts Vrs_3_T3 :: "('a::var, 'b, 'c::var, 'd, 'e, 'f) T3 \<Rightarrow> 'b set"
+consts Vrs_4_T3 :: "('a::var, 'b, 'c::var, 'd, 'e, 'f) T3 \<Rightarrow> 'c set"
+consts Inj_1_T3 :: "'a \<Rightarrow> ('a::var, 'b, 'c::var, 'd, 'e, 'f) T3"
+consts Inj_2_T3 :: "'b \<Rightarrow> ('a::var, 'b, 'c::var, 'd, 'e, 'f) T3"
+
+consts Sb_T4 :: "('a::var \<Rightarrow> ('a, 'b) T4) \<Rightarrow> ('b::var \<Rightarrow> ('a, 'b) T4) \<Rightarrow> ('a, 'b) T4 \<Rightarrow> ('a, 'b) T4"
+consts Vrs_1_T4 :: "('a::var, 'b::var) T4 \<Rightarrow> 'a set"
+consts Vrs_2_T4 :: "('a::var, 'b::var) T4 \<Rightarrow> 'b set"
+consts Inj_1_T4 :: "'a \<Rightarrow> ('a::var, 'b::var) T4"
+consts Inj_2_T4 :: "'b \<Rightarrow> ('a::var, 'b::var) T4"
+
+ML \<open>
+Multithreading.parallel_proofs := 0
+\<close>
+declare [[goals_limit=1000]]
+pbmv_monad "('a, 'b, 'c, 'd, 'e, 'f, 'g) T1"
+  Sbs: Sb_T1
+  RVrs: Vrs_1_T1
+  Injs: Inj_1_T1 Inj_2_T1
+  Vrs: Vrs_2_T1 Vrs_3_T1
+  Maps: Map_T1
+  Supps: set_1_T1 set_2_T1 set_3_T1
+  bd: natLeq
+                      apply (tactic \<open>Skip_Proof.cheat_tac @{context} 1\<close>)+
+  done
+print_theorems
+
+pbmv_monad "('a, 'b, 'c, 'd) T2"
+  Sbs: Sb_T2
+  RVrs: Vrs_1_T2
+  Injs: Inj_T2
+  Vrs: Vrs_2_T2
+  bd: natLeq
+                      apply (tactic \<open>Skip_Proof.cheat_tac @{context} 1\<close>)+
+  done
+
+pbmv_monad "('a, 'b, 'c, 'd, 'e, 'f) T3" and "('a, 'c) T4"
+  Sbs: Sb_T3 and Sb_T4
+  Injs: Inj_1_T3 Inj_1_T4 Inj_2_T3 Inj_2_T4 and Inj_1_T4 Inj_2_T4
+  Vrs: Vrs_1_T3 Vrs_2_T3 Vrs_3_T3 Vrs_4_T3 and Vrs_1_T4 Vrs_2_T4
+  Maps: Map_T3
+  Supps: set_1_T3 set_2_T3
+  bd: natLeq
+                      apply (tactic \<open>Skip_Proof.cheat_tac @{context} 1\<close>)+
+  done
+print_theorems
+print_pbmv_monads
+
+type_synonym ('a, 'b, 'c, 'd, 'e, 'f, 'g, 'h) T =
+  "(('a, 'b, 'e, 'd) T2, 'b, 'c, 'g set, ('b, 'a, 'c, 'd, 'e, 'h) T3, 'f, 'g) T1"
+
+(*
+deads: 'a, 'e, 'f, 'g
+frees: 'b, 'c, 'd
+lives: 'h
+*)
+
+lemma cong': "f x = g x \<Longrightarrow> x = y \<Longrightarrow> f x = g y"
+  by simp
+
+(* Demoting T3 *)
+pbmv_monad T3': "('a, 'b, 'c, 'd, 'e, 'f) T3" and "('a::var, 'c::var) T4"
+  Sbs: "\<lambda>f1 \<rho>1 \<rho>2 \<rho>4. Sb_T3 \<rho>1 \<rho>2 Inj_2_T3 \<rho>4 \<circ> Map_T3 f1 id" and Sb_T4
+  RVrs: set_1_T3
+  Injs: Inj_1_T3 Inj_1_T4 Inj_2_T4 and Inj_1_T4 Inj_2_T4
+  Vrs: Vrs_1_T3 Vrs_2_T3 Vrs_4_T3 and Vrs_1_T4 Vrs_2_T4
+  Maps: "Map_T3 id"
+  Supps: set_2_T3
+  bd: natLeq
+                      apply (rule infinite_regular_card_order_natLeq)
+                      apply (unfold T3.Sb_Inj T3.Map_id id_o)
+                      apply (rule refl)
+                      apply (unfold comp_assoc T3.Map_Inj)
+                      apply (rule T3.Sb_comp_Inj; (assumption | rule SSupp_Inj_bound))+
+                      apply (rule trans)
+                      apply (rule arg_cong2[OF refl, of _ _ "(\<circ>)"])
+                      apply (rule trans[OF comp_assoc[symmetric]])
+                      apply (rule arg_cong2[OF _ refl, of _ _ "(\<circ>)"])
+                      apply (rule T3.Map_Sb)
+                      apply (assumption | rule SSupp_Inj_bound)+
+                      apply (rule trans)
+                      apply (unfold comp_assoc)[1]
+                      apply (rule trans[OF comp_assoc[symmetric]])
+                      apply (rule arg_cong2[of _ _ _ _ "(\<circ>)"])
+                      apply (rule T3.Sb_comp)
+                      apply (assumption | rule T3.SSupp_Map_bound SSupp_Inj_bound)+
+                      apply (rule T3.Map_comp)
+                      apply (unfold id_o T3.Map_Inj)
+                      apply (subst T3.Sb_comp_Inj, (assumption | rule SSupp_Inj_bound)+)+
+                      apply (rule refl)
+
+                      apply (rule T3.Supp_bd T3.Vrs_bd T3.Vrs_Inj)+
+
+  subgoal for f \<rho>1 \<rho>2 \<rho>3 x
+    apply (unfold comp_def)
+    apply (subst T3.Supp_Sb)
+    apply (assumption | rule SSupp_Inj_bound)+
+    apply (rule T3.Supp_Map)
+    done
+  subgoal for f \<rho>1 \<rho>2 \<rho>3 x
+    apply (unfold comp_def)
+    apply (rule trans)
+     apply (rule T3.Vrs_Sb)
+        apply (assumption | rule SSupp_Inj_bound)+
+    apply (unfold T3.Vrs_Map T3.Vrs_Inj UN_empty2 Un_empty_right Un_empty_left)
+    apply (rule refl)
+    done
+
+  subgoal for f \<rho>1 \<rho>2 \<rho>3 x
+    apply (unfold comp_def)
+    apply (rule trans)
+     apply (rule T3.Vrs_Sb)
+        apply (assumption | rule SSupp_Inj_bound)+
+    apply (unfold T3.Vrs_Map T3.Vrs_Inj UN_empty2 Un_empty_right Un_empty_left)
+    apply (rule refl)
+    done
+
+  subgoal for f \<rho>1 \<rho>2 \<rho>3 x
+    apply (unfold comp_def)
+    apply (rule trans)
+     apply (rule T3.Vrs_Sb)
+        apply (assumption | rule SSupp_Inj_bound)+
+    apply (unfold T3.Vrs_Map T3.Vrs_Inj UN_empty2 Un_empty_right Un_empty_left)
+    apply (rule refl)
+    done
+
+  subgoal for f \<rho>1 \<rho>2 \<rho>3 g \<rho>'1 \<rho>'2 \<rho>'3 x
+    apply (rule comp_apply_eq)
+    apply (rule cong'[OF _ T3.Map_cong, rotated])
+      apply (assumption | rule refl)+
+    apply (rule T3.Sb_cong)
+    apply (unfold T3.Vrs_Map)
+               apply (assumption | rule SSupp_Inj_bound refl)+
+    done
+                      apply (rule refl)
+                      apply (rule trans)
+                      apply (rule T3.Map_comp)
+                      apply (unfold id_o)
+                      apply (rule refl)
+                      apply (rule T3.Supp_Map)
+                      apply (rule T3.Supp_bd)
+                      apply (rule T3.Map_cong)
+                      apply (rule refl)
+                      apply assumption
+
+  subgoal for f fa \<rho>1 \<rho>2 \<rho>3
+    apply (rule trans)
+     apply (rule trans[OF comp_assoc[symmetric]])
+     apply (rule arg_cong2[OF _ refl, of _ _ "(\<circ>)"])
+     apply (rule T3.Map_Sb)
+        apply (assumption | rule SSupp_Inj_bound)+
+    apply (unfold T3.Map_Inj comp_assoc)
+    apply (rule arg_cong2[OF refl, of _ _ "(\<circ>)"])
+    apply (rule trans)
+     apply (rule T3.Map_comp)
+    apply (rule sym)
+    apply (rule trans)
+     apply (rule T3.Map_comp)
+    apply (unfold id_o o_id)
+    apply (rule refl)
+    done
+
+                    apply (unfold comp_def)[1]
+                    apply (subst T3.Supp_Sb, (assumption | rule SSupp_Inj_bound)+)
+                    apply (rule trans)
+                     apply (rule T3.Supp_Map)
+                    apply (rule image_id)
+  apply (rule trans)
+                     apply (rule T3.Supp_Map)
+                   apply (rule image_id)
+                  apply (unfold T3.Vrs_Map)
+                  apply (rule refl)+
+             apply (rule T3.Sb_comp_Inj; assumption)+
+           apply (rule T3.Sb_comp; assumption)
+          apply (rule T3.Vrs_bd T3.Vrs_Inj)+
+    apply (rule T3.Vrs_Sb; assumption)+
+  apply (rule T3.Sb_cong; assumption)
+  done
+print_theorems
+
+abbreviation "Vrs_1_T \<equiv> Vrs_2_T1"
+abbreviation "Vrs_2_T \<equiv> \<lambda>x. \<Union> (Vrs_2_T2 ` set_1_T1 x)"
+abbreviation "Vrs_3_T \<equiv> \<lambda>x. \<Union> (Vrs_1_T3 ` set_3_T1 x)"
+
+declare [[ML_print_depth=1000]]
+pbmv_monad T: "('a, 'b, 'c, 'd, 'e, 'f, 'g, 'h) T" and "('a, 'b, 'e, 'd) T2" and T3': "('b, 'a, 'c, 'd, 'e, 'h) T3"
+  Sbs: "\<lambda>h1 h2 \<rho>1 \<rho>2 \<rho>3 \<rho>4 \<rho>5. Sb_T1 h1 \<rho>1 Inj_2_T1 \<circ> Map_T1 (Sb_T2 h2 \<rho>2) id (Sb_T3 \<rho>3 \<rho>4 Inj_2_T3 \<rho>5 \<circ> Map_T3 h2 id)"
+  RVrs: Vrs_1_T1 "\<lambda>x. \<Union> (Vrs_1_T2 ` set_1_T1 x) \<union> \<Union> (set_1_T3 ` set_3_T1 x)"
+  Injs: Inj_1_T1 Inj_T2 Inj_1_T3 Inj_1_T4 Inj_2_T4
+  Vrs: Vrs_2_T1 "\<lambda>x. \<Union> (Vrs_2_T2 ` set_1_T1 x)" "\<lambda>x. \<Union> (Vrs_1_T3 ` set_3_T1 x)" "\<lambda>x. \<Union> (Vrs_2_T3 ` set_3_T1 x)" "\<lambda>x. \<Union> (Vrs_4_T3 ` set_3_T1 x)"
+  Maps: "\<lambda>f. Map_T1 id id (Map_T3 id f)"
+  Supps: "\<lambda>x. \<Union> (set_2_T3 ` set_3_T1 x)"
+  bd: natLeq
+                      apply (rule infinite_regular_card_order_natLeq)
+  subgoal
+    apply (unfold id_o T1.Sb_Inj T1.Map_id T2.Sb_Inj T3.Sb_Inj T3.Map_id)
+    apply (rule refl)
+    done
+  subgoal for f1 f2 \<rho>1 \<rho>2 \<rho>3 \<rho>4 \<rho>5
+    apply (rule trans)
+     apply (rule trans[OF comp_assoc])
+     apply (rule arg_cong2[OF refl, of _ _ "(\<circ>)"])
+    apply (rule T1.Map_Inj)
+     apply (rule T1.Sb_comp_Inj)
+       apply (assumption | rule T1.SSupp_Map_bound SSupp_Inj_bound)+
+    done
+
+  subgoal for g1 g2 \<rho>'1 \<rho>'2 \<rho>'3 \<rho>'4 \<rho>'5 f1 f2 \<rho>1 \<rho>2 \<rho>3 \<rho>4 \<rho>5
+    apply (rule trans)
+     apply (rule trans[OF comp_assoc])
+    apply (rule trans)
+     apply (rule arg_cong2[OF refl, of _ _ "(\<circ>)"])
+     apply (rule trans[OF comp_assoc[symmetric]])
+    apply (rule trans)
+     apply (rule arg_cong2[OF _ refl, of _ _ "(\<circ>)"])
+     apply (rule T1.Map_Sb)
+        apply (assumption | rule SSupp_Inj_bound)+
+     apply (rule trans[OF comp_assoc])
+     apply (rule arg_cong2[OF refl, of _ _ "(\<circ>)"])
+    apply (rule T1.Map_comp)
+     apply (rule comp_assoc[symmetric])
+    apply (subst T1.Sb_comp)
+          apply (assumption | rule T1.SSupp_Map_bound SSupp_Inj_bound)+
+    apply (rule arg_cong2[of _ _ _ _ "(\<circ>)"])
+     apply (rule ext)
+     apply (rule T1.Sb_cong)
+    apply (unfold comp_assoc T1.Map_Inj id_o o_id)
+             apply (assumption | rule supp_comp_bound infinite_UNIV T1.SSupp_Sb_bound SSupp_Inj_bound T1.SSupp_Map_bound refl
+              T1.Sb_comp_Inj[THEN fun_cong]
+            )+
+    apply (rule ext)
+    apply (rule T1.Map_cong)
+      (* REPEAT for inner *)
+      apply (rule T2.Sb_comp[THEN fun_cong], assumption+)
+     apply (rule refl)
+    (* repeated *)
+    apply (rule trans)
+     apply (rule arg_cong2[OF refl, of _ _ "(\<circ>)", THEN fun_cong])
+    apply (rule trans)
+     apply (rule trans[OF comp_assoc[symmetric]])
+     apply (rule arg_cong2[OF _ refl, of _ _ "(\<circ>)"])
+     apply (rule T3.Map_Sb)
+        apply (assumption | rule SSupp_Inj_bound)+
+     apply (unfold T3.Map_Inj)
+     apply (rule trans[OF comp_assoc])
+     apply (rule arg_cong2[OF refl, of _ _ "(\<circ>)"])
+     apply (rule T3.Map_comp)
+    apply (unfold id_o o_id comp_assoc[symmetric])
+    apply (rule arg_cong2[OF _ refl, of _ _ "(\<circ>)", THEN fun_cong])
+    apply (rule trans)
+     apply (rule T3.Sb_comp)
+            apply (assumption | rule T3.SSupp_Map_bound SSupp_Inj_bound)+
+    apply (subst T3.Sb_comp_Inj, (assumption | rule SSupp_Inj_bound)+)+
+    apply (unfold comp_assoc[symmetric])
+    apply (rule refl)
+    done
+
+  apply (unfold T1.Supp_Inj UN_empty)
+  apply (rule refl T1.Vrs_bd T2.Vrs_bd T3.Vrs_bd T1.Vrs_Inj T3'.Vrs_bd infinite_regular_card_order_Un infinite_regular_card_order_UN infinite_regular_card_order_natLeq T1.Supp_bd)+
+
+                      apply (unfold0 comp_apply)[1]
+                      apply (rule trans)
+                      apply (rule T1.Vrs_Sb)
+                      apply (assumption | rule SSupp_Inj_bound)+
+                      apply (unfold T1.Vrs_Map)[1]
+                      apply (rule refl)
+
+                      apply (unfold0 comp_apply)[1]
+                      apply (subst T1.Supp_Sb, (assumption | rule SSupp_Inj_bound)+)+
+                      apply (unfold T1.Supp_Map image_comp[unfolded comp_def] T2.Vrs_Sb image_UN)[1]
+                      apply (subst T3'.Vrs_Sb, (assumption | rule SSupp_Inj_bound)+)+
+                      apply (unfold image_Un image_UN)[1]
+                      apply (rule refl)
+
+  subgoal for f1 f2 \<rho>1 \<rho>2 \<rho>3 \<rho>4 \<rho>5 x
+    apply (unfold0 comp_apply)
+    apply (subst T1.Vrs_Sb)
+       apply (assumption | rule SSupp_Inj_bound)+
+    apply (unfold T1.Vrs_Map T1.Vrs_Inj UN_empty2 Un_empty_right)
+    apply (rule refl)
+    done
+
+  subgoal for f1 f2 \<rho>1 \<rho>2 \<rho>3 \<rho>4 \<rho>5 x
+    apply (unfold0 comp_apply)
+    apply (subst T1.Vrs_Sb T1.Supp_Sb, (assumption | rule SSupp_Inj_bound)+)+
+    apply (unfold T1.Vrs_Map T1.Vrs_Inj T1.Supp_Map image_comp[unfolded comp_def] UN_empty2 Un_empty_right)
+    apply (subst T2.Vrs_Sb T1.Supp_Sb, (assumption | rule SSupp_Inj_bound)+)+
+    apply (unfold UN_UN_flatten)
+    apply (rule refl)
+    done
+
+  subgoal for f1 f2 \<rho>1 \<rho>2 \<rho>3 \<rho>4 \<rho>5 x
+    apply (unfold0 comp_apply)
+    apply (subst T1.Vrs_Sb T1.Supp_Sb, (assumption | rule SSupp_Inj_bound)+)+
+    apply (unfold T1.Vrs_Map T1.Vrs_Inj comp_apply T1.Supp_Map image_comp[unfolded comp_def] UN_empty2 Un_empty_right)
+    apply (subst T3.Vrs_Sb T1.Supp_Sb, (assumption | rule SSupp_Inj_bound)+)+
+    apply (unfold UN_UN_flatten T3.Vrs_Map T3.Vrs_Inj UN_empty2 Un_empty_right)
+    apply (rule refl)
+    done
+
+  subgoal for f1 f2 \<rho>1 \<rho>2 \<rho>3 \<rho>4 \<rho>5 x
+    apply (unfold0 comp_apply)
+    apply (subst T1.Vrs_Sb T1.Supp_Sb, (assumption | rule SSupp_Inj_bound)+)+
+    apply (unfold T1.Vrs_Map T1.Vrs_Inj comp_apply T1.Supp_Map image_comp[unfolded comp_def] UN_empty2 Un_empty_right)
+    apply (subst T3.Vrs_Sb T1.Supp_Sb, (assumption | rule SSupp_Inj_bound)+)+
+    apply (unfold UN_UN_flatten T3.Vrs_Map T3.Vrs_Inj UN_empty2 Un_empty_right UN_Un_distrib)
+    apply (rule refl)
+    done
+
+  subgoal for f1 f2 \<rho>1 \<rho>2 \<rho>3 \<rho>4 \<rho>5 x
+    apply (unfold0 comp_apply)
+    apply (subst T1.Vrs_Sb T1.Supp_Sb, (assumption | rule SSupp_Inj_bound)+)+
+    apply (unfold T1.Vrs_Map T1.Vrs_Inj comp_apply T1.Supp_Map image_comp[unfolded comp_def] UN_empty2 Un_empty_right)
+    apply (subst T3.Vrs_Sb T1.Supp_Sb, (assumption | rule SSupp_Inj_bound)+)+
+    apply (unfold UN_UN_flatten T3.Vrs_Map T3.Vrs_Inj UN_empty2 Un_empty_right UN_Un_distrib)
+    apply (rule refl)
+    done
+
+  subgoal premises prems for f1 f2 \<rho>1 \<rho>2 \<rho>3 \<rho>4 \<rho>5 g1 g2 \<rho>'1 \<rho>'2 \<rho>'3 \<rho>'4 \<rho>'5 x
+    apply (rule comp_apply_eq)
+    apply (rule cong'[OF _ T1.Map_cong, rotated])
+    (* REPEAT for inners *)
+       apply (rule T2.Sb_cong)
+            apply (rule prems)+
+  (* REPEAT_DETERM *)
+        apply (drule UN_I)
+         apply assumption
+        apply (assumption | erule UnI1 UnI2 | rule UnI2)+
+    (* repeated *)
+    apply (rule prems)
+        apply (drule UN_I)
+         apply assumption
+        apply (assumption | erule UnI1 UnI2 | rule UnI2)+
+    (* END REPEAT_DETERM *)
+  (* second inner *)
+      apply (rule refl)
+  (* third inner *)
+     apply (rule T3'.Sb_cong)
+    apply (rule prems)+
+  (* REPEAT_DETERM *)
+        apply (drule UN_I)
+         apply assumption
+        apply (assumption | erule UnI1 UnI2 | rule UnI2)+
+    (* repeated *)
+    apply (rule prems)
+        apply (drule UN_I)
+         apply assumption
+        apply (assumption | erule UnI1 UnI2 | rule UnI2)+
+    (* repeated *)
+    apply (rule prems)
+        apply (drule UN_I)
+         apply assumption
+        apply (assumption | erule UnI1 UnI2 | rule UnI2)+
+    (* repeated *)
+    apply (rule prems)
+        apply (drule UN_I)
+         apply assumption
+     apply (assumption | erule UnI1 UnI2 | rule UnI2)+
+  (* END REPEAT_DETERM *)
+    apply (rule T1.Sb_cong)
+    apply (unfold T1.Vrs_Map)
+            apply (rule prems SSupp_Inj_bound refl | assumption| erule UnI1 UnI2 | rule UnI2)+
+    done
+
+                apply (unfold T3'.Map_id T1.Map_id)[1]
+                apply (rule refl)
+
+               apply (unfold T1.Map_comp id_o o_id T3'.Map_comp)[1]
+               apply (rule refl)
+
+              apply (unfold T1.Supp_Map image_comp[unfolded comp_def] T3'.Supp_Map image_UN)[1]
+              apply (rule refl)
+
+             apply (rule infinite_regular_card_order_UN infinite_regular_card_order_natLeq T1.Supp_bd T3'.Supp_bd)+
+
+  subgoal premises prems for f g x
+    apply (rule T1.Map_cong)
+      apply (rule refl)+
+    apply (rule T3'.Map_cong)
+    apply (rule prems)
+    apply (erule UN_I)
+    apply assumption
+    done
+
+  subgoal for f f1 f2 \<rho>1 \<rho>2 \<rho>3 \<rho>4 \<rho>5
+    apply (unfold comp_assoc[symmetric])
+    apply (rule trans)
+     apply (rule arg_cong2[OF T1.Map_Sb refl])
+       apply (assumption | rule SSupp_Inj_bound)+
+    apply (unfold T1.Map_Inj comp_assoc T1.Map_comp id_o o_id T3'.Map_Sb)
+    apply (rule refl)
+    done
+
+  apply (unfold0 comp_apply)[1]
+          apply (subst T1.Supp_Sb, (assumption | rule SSupp_Inj_bound)+)+
+          apply (unfold T1.Supp_Map image_comp[unfolded comp_def] T3'.Supp_Sb)[1]
+          apply (rule refl)
+
+         apply (unfold T1.Vrs_Map T1.Supp_Map image_id image_comp[unfolded comp_def] T3'.Vrs_Map T1.Map_Inj)
+         apply (rule refl)+
+  done
+print_theorems
+
+ML \<open>
+val T1 = the (BMV_Monad_Def.pbmv_monad_of @{context} @{type_name T1});
+val T2 = the (BMV_Monad_Def.pbmv_monad_of @{context} @{type_name T2});
+val T3 = the (BMV_Monad_Def.pbmv_monad_of @{context} "BMV_Composition.T3'");
+\<close>
+
+local_setup \<open>fn lthy =>
+let
+  open MRBNF_Util
+  val ((bmv, unfold_set), lthy) = BMV_Monad_Def.compose_bmv_monad I T1 [Inl T2, Inr @{typ "'g set"}, Inl T3]
+    { frees = [@{typ 'b}, @{typ 'c}, @{typ 'g}], deads = [@{typ 'f}] }
+    [ SOME { frees = [@{typ 'd}, @{typ 'b}], lives = [], deads = [@{typ 'a}, @{typ 'e}] },
+      NONE,
+      SOME { frees = [@{typ 'b}, @{typ 'a}, @{typ 'c}], lives = [@{typ 'd}, @{typ 'h}], deads = [@{typ 'e}] }
+    ] lthy
+in lthy end
+\<close>
+
 
 end
